libcrux-ml-dsa/proofs/fstar/spec/Spec.Intrinsics.fsti
@@ -2,6 +2,43 @@ module Spec.Intrinsics
 open Core
 open Core_models.Core_arch.X86.Interpretations.Int_vec
 
+(* Opaque arithmetic operations *)
+[@@ "opaque_to_smt"]
+let add_mod_opaque #t = add_mod #t
+
+[@@ "opaque_to_smt"]
+let sub_mod_opaque #t = sub_mod #t
+
+[@@ "opaque_to_smt"]
+let mul_mod_opaque #t = mul_mod #t
+
+[@@ "opaque_to_smt"]
+let shift_right_opaque #t = shift_right #t #i32_inttype
+
+[@@ "opaque_to_smt"]
+let shift_left_opaque #t = shift_left #t #i32_inttype
+
+[@@ "opaque_to_smt"]
+let cast_mod_opaque #t #t' = cast_mod #t #t'
+
+let reveal_opaque_arithmetic_ops #t:
+  Lemma (add_mod_opaque #t == add_mod #t /\
+         sub_mod_opaque #t == sub_mod #t /\
+         mul_mod_opaque #t == mul_mod #t /\
+         shift_left_opaque #t == shift_left #t #i32_inttype /\
+         shift_right_opaque #t == shift_right #t #i32_inttype) =
+  reveal_opaque (`%add_mod_opaque) (add_mod_opaque #t);
+  reveal_opaque (`%sub_mod_opaque) (sub_mod_opaque #t);
+  reveal_opaque (`%mul_mod_opaque) (mul_mod_opaque #t);
+  reveal_opaque (`%shift_left_opaque) (shift_left_opaque #t);
+  reveal_opaque (`%shift_right_opaque) (shift_right_opaque #t)
+  
+let reveal_opaque_cast_ops #t #t':
+  Lemma (cast_mod_opaque #t #t' == cast_mod #t #t' /\
+         cast_mod_opaque #t' #t == cast_mod #t' #t) =
+  reveal_opaque (`%cast_mod_opaque) (cast_mod_opaque #t #t');
+  reveal_opaque (`%cast_mod_opaque) (cast_mod_opaque #t' #t)
+
 open FStar.FunctionalExtensionality
 type t_FunArray (n: u64) t = i:u64 {v i < v n} ^-> t
 
@@ -30,22 +67,42 @@ val mm256_shuffle_epi32_lemma (a:i32) (b:bv256) (i:u64{v i < 8}):
 
 val mm256_sub_epi32_lemma (a b: bv256) (i:u64{v i < 8}):
   Lemma (to_i32x8 (Libcrux_intrinsics.Avx2.mm256_sub_epi32 a b) i ==
-         sub_mod (to_i32x8 a i) (to_i32x8 b i))
+         sub_mod_opaque (to_i32x8 a i) (to_i32x8 b i))
          [SMTPat (to_i32x8 (Libcrux_intrinsics.Avx2.mm256_sub_epi32 a b) i)]
 
 val mm256_add_epi32_lemma (a b: bv256) (i:u64{v i < 8}):
   Lemma (to_i32x8 (Libcrux_intrinsics.Avx2.mm256_add_epi32 a b) i ==
-         add_mod (to_i32x8 a i) (to_i32x8 b i))
+         add_mod_opaque (to_i32x8 a i) (to_i32x8 b i))
          [SMTPat (to_i32x8 (Libcrux_intrinsics.Avx2.mm256_add_epi32 a b) i)]
 
-val mm256_mul_Sepi32_lemma (a b: bv256) (i:u64{v i < 8}):
+val mm256_mul_epi32_lemma (a b: bv256) (i:u64{v i < 8}):
   Lemma (to_i32x8 (Libcrux_intrinsics.Avx2.mm256_mul_epi32 a b) i ==
          (
            let j = i /! mk_int 2 in
-           let v64 = (cast (to_i32x8 a j) <: i64) *! (cast (to_i32x8 b j) <: i64) in
-           if v i % 2 = 0 then cast (v64 >>! mk_u64 32) else cast v64
+           let v64 = mul_mod_opaque (cast_mod_opaque (to_i32x8 a j) <: i64) (cast_mod_opaque (to_i32x8 b j) <: i64) in
+           if v i % 2 = 0 then cast_mod_opaque v64 else cast_mod_opaque (shift_right_opaque v64 (mk_i32 32))
          ))
          [SMTPat (to_i32x8 (Libcrux_intrinsics.Avx2.mm256_mul_epi32 a b) i)]
+
+
+val mm256_srai_epi32_lemma (v_IMM8: i32) (a: bv256) (i:u64{v i < 8}):
+  Lemma (to_i32x8 (Libcrux_intrinsics.Avx2.mm256_srai_epi32 v_IMM8 a) i ==
+         (
+         let imm8:i32 = Core.Num.impl_i32__rem_euclid v_IMM8 (mk_i32 256) in
+         if imm8 >. mk_i32 31
+         then if (to_i32x8 a i) <. mk_i32 0 then mk_i32 (-1) else mk_i32 0
+         else shift_right_opaque (to_i32x8 a i) imm8
+         ))
+         [SMTPat (to_i32x8 (Libcrux_intrinsics.Avx2.mm256_srai_epi32 v_IMM8 a) i)]
+
+val mm256_and_si256_lemma (a b: bv256) (i:u64{v i < 8}):
+  Lemma (to_i32x8 (Libcrux_intrinsics.Avx2.mm256_add_epi32 a b) i ==
+         ((to_i32x8 a i) &. (to_i32x8 b i)))
+         [SMTPat (to_i32x8 (Libcrux_intrinsics.Avx2.mm256_and_si256 a b) i)]
+
+val mm256_set1_epi32_lemma (x:i32) (i:u64{v i < 8}):
+  Lemma (to_i32x8 (Libcrux_intrinsics.Avx2.mm256_set1_epi32 x) i == x)
+        [SMTPat (to_i32x8 (Libcrux_intrinsics.Avx2.mm256_set1_epi32 x) i)]
 
 val mm256_set_epi32_lemma (x0 x1 x2 x3 x4 x5 x6 x7:i32) (i:u64{v i < 8}):
   Lemma (to_i32x8 (Libcrux_intrinsics.Avx2.mm256_set_epi32 x0 x1 x2 x3 x4 x5 x6 x7) i ==
@@ -69,9 +126,10 @@ val mm256_set_epi32_lemma (x0 x1 x2 x3 x4 x5 x6 x7:i32) (i:u64{v i < 8}):
 
 val mm256_blend_epi32_lemma (imm8: i32) (a b: bv256) (i:u64{v i < 8}):
   Lemma (to_i32x8 (Libcrux_intrinsics.Avx2.mm256_blend_epi32 imm8 a b) i ==
-        (if ((imm8 >>! i <: i32) %! mk_i32 2 <: i32) =. mk_i32 0 <: bool
+        (if (v imm8 / pow2 (v i)) % 2 = 0
          then to_i32x8 a i
          else to_i32x8 b i))
+  [SMTPat (to_i32x8 (Libcrux_intrinsics.Avx2.mm256_blend_epi32 imm8 a b) i)]
 
 val mm256_set_m128i_lemma (hi lo: bv128) (i:u64{v i < 8}):
   Lemma (to_i32x8 (Libcrux_intrinsics.Avx2.mm256_set_m128i hi lo) i ==
@@ -154,38 +212,3 @@ val mm256_unpackhi_epi64_lemma (a b: bv256) (i:u64{v i < 8}):
           <:
           i32))
   [SMTPat (to_i32x8 (Libcrux_intrinsics.Avx2.mm256_unpackhi_epi64 a b) i)]
-
-val montgomery_multiply_aux_lemma field_modulus inverse_of_modulus_mod_montgomery_r
-  (a b: Core_models.Abstractions.Bitvec.t_BitVec (mk_u64 256))
-  (i:u64{v i < 8}):
-  Lemma 
-    (requires
-        field_modulus ==
-        (Libcrux_intrinsics.Avx2.mm256_set1_epi32 Libcrux_ml_dsa.Simd.Traits.v_FIELD_MODULUS
-          <:
-          Core_models.Abstractions.Bitvec.t_BitVec (mk_u64 256)) /\
-        inverse_of_modulus_mod_montgomery_r ==
-        (Libcrux_intrinsics.Avx2.mm256_set1_epi32 (cast (Libcrux_ml_dsa.Simd.Traits.v_INVERSE_OF_MODULUS_MOD_MONTGOMERY_R
-                  <:
-                  u64)
-              <:
-              i32)
-          <:
-          Core_models.Abstractions.Bitvec.t_BitVec (mk_u64 256)))
-  (ensures
-    to_i32x8 (Libcrux_ml_dsa.Simd.Avx2.Arithmetic.montgomery_multiply_aux field_modulus inverse_of_modulus_mod_montgomery_r a b) i ==
-    Spec.MLDSA.Math.mont_mul (to_i32x8 a i) (to_i32x8 b i))
-    [SMTPat (to_i32x8 (Libcrux_ml_dsa.Simd.Avx2.Arithmetic.montgomery_multiply_aux field_modulus inverse_of_modulus_mod_montgomery_r a b) i)]
-
-let montgomery_multiply_lemma
-  (a b: Core_models.Abstractions.Bitvec.t_BitVec (mk_u64 256))
-  (i:u64{v i < 8}):
-  Lemma (
-    to_i32x8 (Libcrux_ml_dsa.Simd.Avx2.Arithmetic.montgomery_multiply a b) i ==
-    Spec.MLDSA.Math.mont_mul (to_i32x8 a i) (to_i32x8 b i))
-    [SMTPat (to_i32x8 (Libcrux_ml_dsa.Simd.Avx2.Arithmetic.montgomery_multiply a b) i)]
-   =
-   reveal_opaque (`%Libcrux_ml_dsa.Simd.Avx2.Arithmetic.montgomery_multiply) (Libcrux_ml_dsa.Simd.Avx2.Arithmetic.montgomery_multiply)
-
-
-
